Put marshalling

src/program_proof/memkv/memkv_marshal_put_proof.v
@@ -1,3 +1,4 @@
+From Perennial.Helpers Require Import ModArith.
 From Perennial.program_proof Require Import dist_prelude.
 From Goose.github_com.mit_pdos.gokv Require Import memkv.
 From Perennial.program_proof Require Import marshal_proof.
@@ -27,7 +28,7 @@ Definition own_PutRequest args_ptr val_sl args : iProp Σ :=
   "HSeq" ∷ args_ptr ↦[PutRequest :: "Seq"] #args.(PR_Seq) ∗
   "HKey" ∷ args_ptr ↦[PutRequest :: "Key"] #args.(PR_Key) ∗
   "HValue" ∷ args_ptr ↦[PutRequest :: "Value"] (slice_val val_sl) ∗
-  "HValue_sl" ∷ typed_slice.is_slice val_sl byteT 1%Qp args.(PR_Value) ∗
+  "#HValue_sl" ∷ readonly (typed_slice.is_slice_small val_sl byteT 1 args.(PR_Value)) ∗
   "%HseqPositive" ∷ ⌜int.Z args.(PR_Seq) > 0⌝
 .
 
@@ -36,7 +37,8 @@ Definition own_PutReply reply_ptr rep : iProp Σ :=
 .
 
 Definition has_encoding_PutRequest (data:list u8) (args:PutRequestC) : Prop :=
-  has_encoding data [ EncUInt64 args.(PR_CID) ; EncUInt64 args.(PR_Seq); EncUInt64 args.(PR_Key); EncUInt64 (length args.(PR_Value)) ; EncBytes args.(PR_Value) ].
+  has_encoding data [ EncUInt64 args.(PR_CID) ; EncUInt64 args.(PR_Seq); EncUInt64 args.(PR_Key); EncUInt64 (length args.(PR_Value)) ; EncBytes args.(PR_Value) ] ∧
+  int.Z args.(PR_Seq) > 0.
 
 Definition has_encoding_PutReply (data:list u8) (rep:PutReplyC) :=
   has_encoding data [ EncUInt64 rep.(PR_Err) ].
@@ -52,7 +54,72 @@ Lemma wp_encodePutRequest args_ptr val_sl args :
                                                own_PutRequest args_ptr val_sl args
   }}}.
 Proof.
-Admitted.
+  iIntros (Φ) "Hrep HΦ".
+
+  wp_lam.
+  wp_pures.
+  iNamed "Hrep".
+  wp_loadField.
+  wp_apply (wp_slice_len).
+  wp_pures.
+
+  wp_loadField.
+  wp_apply (wp_slice_len).
+  wp_apply (wp_Assume).
+  rewrite bool_decide_eq_true.
+  iIntros (Hoverflow).
+  apply sum_nooverflow_r in Hoverflow.
+  change (int.Z (word.add (word.add (word.add 8 8) 8) 8)) with 32%Z in Hoverflow.
+
+  wp_apply (wp_new_enc).
+  iIntros (enc) "Henc".
+  wp_pures.
+
+  wp_loadField.
+  wp_apply (wp_Enc__PutInt with "Henc").
+  { word. }
+  iIntros "Henc".
+  wp_pures.
+
+  wp_loadField.
+  wp_apply (wp_Enc__PutInt with "Henc").
+  { word. }
+  iIntros "Henc".
+  wp_pures.
+
+  wp_loadField.
+  wp_apply (wp_Enc__PutInt with "Henc").
+  { word. }
+  iIntros "Henc".
+  wp_pures.
+
+  wp_loadField.
+  iMod (readonly_load with "HValue_sl") as (q) "HValue_sl'".
+  iDestruct (typed_slice.is_slice_small_sz with "HValue_sl'") as %Hsz.
+  wp_apply (wp_slice_len).
+  wp_apply (wp_Enc__PutInt with "Henc").
+  { word. }
+  iIntros "Henc".
+  wp_pures.
+
+  wp_loadField.
+  wp_apply (wp_Enc__PutBytes with "[$Henc $HValue_sl']").
+  { word. }
+  iIntros "[Henc _]".
+  wp_pures.
+
+  wp_apply (wp_Enc__Finish with "Henc").
+  iIntros (rep_sl repData).
+  iIntros "(%Henc & %Hlen & Hrep_sl)".
+  iApply "HΦ".
+  iFrame "∗#".
+  iPureIntro.
+  split; last word.
+  rewrite /has_encoding_PutRequest.
+  split; last done.
+  replace (U64 (length args.(PR_Value))) with val_sl.(Slice.sz); first done.
+  word.
+Qed.
 
 Lemma wp_decodePutRequest req_sl reqData args :
   {{{
@@ -64,20 +131,50 @@ Lemma wp_decodePutRequest req_sl reqData args :
        (args_ptr:loc) val_sl, RET #args_ptr; own_PutRequest args_ptr val_sl args
   }}}.
 Proof.
-Admitted.
+  iIntros (Φ) "[%Henc Hsl] HΦ".
+  wp_lam.
+  wp_apply (wp_allocStruct).
+  {
+    rewrite zero_slice_val.
+    naive_solver.
+  }
+  iIntros (rep_ptr) "Hrep".
+  iDestruct (struct_fields_split with "Hrep") as "HH".
+  iNamed "HH".
+  wp_pures.
 
-Lemma wp_decodePutReply rep rep_sl repData :
-  {{{
-       typed_slice.is_slice rep_sl byteT 1%Qp repData ∗
-       ⌜has_encoding_PutReply repData rep ⌝
-  }}}
-    decodePutReply (slice_val rep_sl)
-  {{{
-       (rep_ptr:loc) , RET #rep_ptr;
-       own_PutReply rep_ptr rep
-  }}}.
-Proof.
-Admitted.
+  iDestruct (typed_slice.is_slice_small_acc with "Hsl") as "[Hsl _]".
+  destruct Henc as [Henc Hseq].
+  wp_apply (wp_new_dec with "[$Hsl]").
+  { done. }
+  iIntros (?) "Hdec".
+  wp_pures.
+
+  wp_apply (wp_Dec__GetInt with "[$Hdec]").
+  iIntros "Hdec".
+  wp_storeField.
+
+  wp_apply (wp_Dec__GetInt with "[$Hdec]").
+  iIntros "Hdec".
+  wp_storeField.
+
+  wp_apply (wp_Dec__GetInt with "[$Hdec]").
+  iIntros "Hdec".
+  wp_storeField.
+
+  wp_apply (wp_Dec__GetInt with "[$Hdec]").
+  iIntros "Hdec".
+  wp_apply (wp_Dec__GetBytes_ro with "[$Hdec]"); first done.
+  iIntros (??) "[Hsl Hdec]".
+  wp_apply (wp_storeField with "Value").
+  { apply slice_val_ty. }
+  iIntros "Value".
+
+  wp_pures.
+  iApply "HΦ".
+  iFrame.
+  iPureIntro. done.
+Qed.
 
 Lemma wp_encodePutReply rep_ptr rep :
   {{{
@@ -90,6 +187,67 @@ Lemma wp_encodePutReply rep_ptr rep :
        ⌜has_encoding_PutReply repData rep ⌝
   }}}.
 Proof.
-Admitted.
+  iIntros (Φ) "Hrep HΦ".
+
+  wp_lam.
+  wp_pures.
+  iNamed "Hrep".
+
+  wp_apply (wp_new_enc).
+  iIntros (enc) "Henc".
+  wp_pures.
+
+  wp_loadField.
+  wp_apply (wp_Enc__PutInt with "Henc").
+  { word. }
+  iIntros "Henc".
+  wp_pures.
+
+  wp_apply (wp_Enc__Finish with "Henc").
+  iIntros (rep_sl repData).
+  iIntros "(%Henc & %Hlen & Hrep_sl)".
+  iApply "HΦ".
+  iFrame.
+  iPureIntro.
+  rewrite /has_encoding_PutReply.
+  done.
+Qed.
+
+Lemma wp_decodePutReply rep rep_sl repData :
+  {{{
+       typed_slice.is_slice rep_sl byteT 1%Qp repData ∗
+       ⌜has_encoding_PutReply repData rep ⌝
+  }}}
+    decodePutReply (slice_val rep_sl)
+  {{{
+       (rep_ptr:loc) , RET #rep_ptr;
+       own_PutReply rep_ptr rep
+  }}}.
+Proof.
+  iIntros (Φ) "[Hsl %Henc] HΦ".
+  wp_lam.
+  wp_apply (wp_allocStruct).
+  {
+    naive_solver.
+  }
+  iIntros (rep_ptr) "Hrep".
+  iDestruct (struct_fields_split with "Hrep") as "HH".
+  iNamed "HH".
+  wp_pures.
+
+  iDestruct (typed_slice.is_slice_small_acc with "Hsl") as "[Hsl _]".
+  wp_apply (wp_new_dec with "[$Hsl]").
+  { done. }
+  iIntros (?) "Hdec".
+  wp_pures.
+
+  wp_apply (wp_Dec__GetInt with "[$Hdec]").
+  iIntros "Hdec".
+  wp_storeField.
+
+  iApply "HΦ".
+  iModIntro.
+  iFrame.
+Qed.
 
 End memkv_marshal_put_proof.
