src/program_proof/memkv/memkv_marshal_get_proof.v
@@ -34,7 +34,7 @@ Definition own_GetReply reply_ptr rep : iProp Σ :=
   ∃ val_sl,
   "HErr" ∷ reply_ptr ↦[GetReply :: "Err"] #rep.(GR_Err) ∗
   "HValue" ∷ reply_ptr ↦[GetReply :: "Value"] (slice_val val_sl) ∗
-  "HValue_sl" ∷ ∃ (q:Qp), (typed_slice.is_slice_small val_sl byteT q rep.(GR_Value))
+  "#HValue_sl" ∷ readonly (typed_slice.is_slice_small val_sl byteT 1 rep.(GR_Value))
 .
 
 Definition has_encoding_GetRequest (data:list u8) (args:GetRequestC) :=
@@ -42,8 +42,7 @@ Definition has_encoding_GetRequest (data:list u8) (args:GetRequestC) :=
   int.Z args.(GR_Seq) > 0.
 
 Definition has_encoding_GetReply (data:list u8) (rep:GetReplyC) :=
-  has_encoding data [ EncUInt64 rep.(GR_Err) ; EncUInt64 (length rep.(GR_Value)) ; EncBytes rep.(GR_Value) ] ∧
-  length rep.(GR_Value) = int.nat (length rep.(GR_Value)).
+  has_encoding data [ EncUInt64 rep.(GR_Err) ; EncUInt64 (length rep.(GR_Value)) ; EncBytes rep.(GR_Value) ].
 
 Lemma wp_encodeGetRequest args_ptr args :
   {{{
@@ -151,8 +150,8 @@ Proof.
   iDestruct (struct_fields_split with "Hrep") as "HH".
   iNamed "HH".
   wp_pures.
+
   iDestruct (typed_slice.is_slice_small_acc with "Hsl") as "[Hsl _]".
-  destruct Henc as [Henc Hsz].
   wp_apply (wp_new_dec with "[$Hsl]").
   { done. }
   iIntros (?) "Hdec".
@@ -164,18 +163,18 @@ Proof.
 
   wp_apply (wp_Dec__GetInt with "[$Hdec]").
   iIntros "Hdec".
-  wp_apply (wp_Dec__GetBytes with "[$Hdec]").
+  wp_apply (wp_Dec__GetBytes_ro with "[$Hdec]").
   { done. }
   iIntros (??) "[Hsl Hdec]".
   wp_apply (wp_storeField with "Value").
   { apply slice_val_ty. }
   iIntros "Value".
+
   wp_pures.
   iApply "HΦ".
   iModIntro.
   iExists _.
-  iFrame.
-  iExists _; iFrame.
+  by iFrame.
 Qed.
 
 Lemma wp_encodeGetReply rep_ptr rep :
@@ -217,8 +216,8 @@ Proof.
   wp_pures.
 
   wp_loadField.
-  iDestruct "HValue_sl" as (?) "HValue_sl".
-  iDestruct (typed_slice.is_slice_small_sz with "HValue_sl") as %Hsz.
+  iMod (readonly_load with "HValue_sl") as (q) "HValue_sl'".
+  iDestruct (typed_slice.is_slice_small_sz with "HValue_sl'") as %Hsz.
   wp_apply (wp_slice_len).
   wp_apply (wp_Enc__PutInt with "Henc").
   { apply dec_stable. intros HP. apply HP. word. }
@@ -226,28 +225,23 @@ Proof.
   wp_pures.
 
   wp_loadField.
-  wp_apply (wp_Enc__PutBytes with "[$Henc $HValue_sl]").
+  wp_apply (wp_Enc__PutBytes with "[$Henc $HValue_sl']").
   { apply sum_nooverflow_r in Hoverflow.
     rewrite Hoverflow Hsz.
     change (int.Z (word.add 8 8)) with 16.
     rewrite Z2Nat.id; word. }
-  iIntros "[Henc Hsl]".
+  iIntros "[Henc _]".
   wp_pures.
+
   wp_apply (wp_Enc__Finish with "[$Henc]").
   iIntros (rep_sl repData).
   iIntros "(% & % & Hrep_sl)".
   iApply "HΦ".
   iFrame.
-  iDestruct (typed_slice.is_slice_small_sz with "Hsl") as %Hsz2.
   iPureIntro.
   unfold has_encoding_GetReply.
-  rewrite Hsz.
-  assert (U64 (int.nat (Slice.sz val_sl)) = (Slice.sz val_sl)).
-  { word. }
-  rewrite H1.
-  rewrite app_nil_l in H.
-  simpl in H.
-  done.
+  replace (U64 (length rep.(GR_Value))) with val_sl.(Slice.sz); first done.
+  word.
 Qed.
 
 End memkv_marshal_get_proof.
